Working on parameterized stacks

755/Project2/Natstack.v
@@ -1,13 +1,11 @@
+Require Import Omega.
+
 (* Lynne Coblammers *)
 (* EECS 755 *)
 (* Mini Project 2 *)
 (* 2015.10.18 *)
 
 (*************************Problem 1**********************)
-Inductive SC : Type :=
-  | Value : nat -> SC
-  | Unknown : SC.
-
 Inductive NatStack : Type :=
   | Empty : NatStack
   | Add : nat -> NatStack -> NatStack.
@@ -19,7 +17,6 @@ Inductive NatStack : Type :=
 *)
 Definition push (n : nat) (s : NatStack) : NatStack :=
   Add n s.
-
 
 (* 
   Preconditions: s is not empty
@@ -53,3 +50,55 @@ Definition isEmpty (s : NatStack) : bool :=
     | Empty => true
     | Add _ _ => false
   end.
+
+Fixpoint size (s : NatStack) : nat :=
+  match s with
+    | Empty => 0
+    | Add _ s => 1 + size s
+  end.
+
+Theorem top_correct : forall n s, top (Add n s) = n.
+Proof.
+  intros.
+  simpl.
+  reflexivity.
+Qed.
+
+Theorem push_immediate : forall n s, top (push n s) = n.
+Proof.
+  intros.
+  simpl.
+  reflexivity.
+Qed.
+
+Theorem push_increase_size : forall n s, size (push n s) = 1 + size s.
+Proof.
+  intros.
+  simpl.
+  reflexivity.
+Qed.
+
+Theorem push_invariant : forall n s, pop (push n s) = s.
+Proof.
+  intros.
+  simpl.
+  reflexivity.
+Qed.
+
+Theorem pop_imediate : forall n s, size (pop (Add n s)) = size s.
+Proof.
+  intros.
+  simpl.
+  reflexivity.
+Qed.
+
+Theorem isEmpty_correct_true : isEmpty(Empty) = true.
+Proof.
+  reflexivity.
+Qed.
+
+Theorem isEmpty_correct_false : forall n s, isEmpty(Add n s) = false.
+Proof.
+  intros.
+  reflexivity.
+Qed.
