755/Project2/ParameterizedStack.v
@@ -1,0 +1,108 @@
+Require Import Omega.
+
+(* Lynne Coblammers *)
+(* EECS 755 *)
+(* Mini Project 2 *)
+(* 2015.10.19 *)
+
+(*************************Problem 2**********************)
+Inductive SC : Type :=
+  | Value : nat -> SC
+  | Unknown : SC.
+
+Inductive Stack : Type :=
+  | Empty : Stack
+  | Add : SC -> Stack -> Stack.
+
+(* 
+  Preconditions: None 
+  Postconditions: n is top of resulting stack
+  Invariants: resulting stack is same as s except for new top element
+*)
+Definition push (v: SC) (s : Stack) : Stack :=
+  Add v s.
+
+(* 
+  Preconditions: s is not empty
+  Postconditions: top element removed from stack
+  Invariants: resulting stack is same except for removed top element
+*)
+Definition pop (s : Stack) : Stack  :=
+  match s with
+    | Empty => Empty
+    | Add v s => s
+  end.
+
+(* 
+  Preconditions: s is not empty
+  Postconditions: SC is top element of stack
+  Invariants: stack is unchanged
+*)
+Definition top (s : Stack) : SC :=
+  match s with
+    | Empty => Unknown
+    | Add v s => v
+  end.
+
+(* 
+  Preconditions: None
+  Postconditions: true if stack is empty, false otherwise
+  Invariants: stack is unchanged
+*)
+Definition isEmpty (s : Stack) : bool :=
+  match s with
+    | Empty => true
+    | Add _ _ => false
+  end.
+
+Fixpoint size (s : Stack) : nat :=
+  match s with
+    | Empty => 0
+    | Add _ s => 1 + size s
+  end.
+
+Theorem top_correct : forall n s, top (Add n s) = n.
+Proof.
+  intros.
+  simpl.
+  reflexivity.
+Qed.
+
+Theorem push_immediate : forall n s, top (push n s) = n.
+Proof.
+  intros.
+  simpl.
+  reflexivity.
+Qed.
+
+Theorem push_increase_size : forall n s, size (push n s) = 1 + size s.
+Proof.
+  intros.
+  simpl.
+  reflexivity.
+Qed.
+
+Theorem push_invariant : forall n s, pop (push n s) = s.
+Proof.
+  intros.
+  simpl.
+  reflexivity.
+Qed.
+
+Theorem pop_imediate : forall v s, size (pop (Add v s)) = size s.
+Proof.
+  intros.
+  simpl.
+  reflexivity.
+Qed.
+
+Theorem isEmpty_correct_true : isEmpty(Empty) = true.
+Proof.
+  reflexivity.
+Qed.
+
+Theorem isEmpty_correct_false : forall n s, isEmpty(Add n s) = false.
+Proof.
+  intros.
+  reflexivity.
+Qed.
